theories/Algebra/AbGroups/AbSES/PullbackFiberSequence.v
@@ -1,0 +1,366 @@
+Require Import Basics Types HSet HFiber Limits.Pullback Cubical.PathSquare.
+Require Import WildCat Pointed Homotopy.ExactSequence.
+Require Import AbGroups.AbelianGroup AbSES.Core AbSES.Pullback.
+Require Import Modalities.Identity.
+
+(** * The fiber sequence induced by pulling back along a short exact sequence *)
+
+(** We show that pulling back along a short exact sequence [E : AbSES C A] produces a fiber sequence [AbSES C A -> AbSES E A -> AbSES B A]. The associated long exact sequence of homotopy groups recovers the usual (contravariant) six-term exact sequence of Ext groups.
+
+We will prove the analog of exactness in terms of path data, and deduce the usual notion. *)
+
+(** If a short exact sequence [A -> F -> B'] becomes trivial after pulling back along an inclusion [i : B -> E], then there is a "transpose" short exact sequence [B -> F -> F/B]. We begin by constructing the endpoint [F/B]. *)
+
+Definition abses_pullback_inclusion_transpose_subgroup `{Univalence} {A B E : AbGroup}
+      (i : B $-> E) `{IsEmbedding i}
+      (F : AbSES E A) (p : abses_pullback0 i F $== point _)
+  : NormalSubgroup F.
+Proof.
+  srapply (ab_image_embedding (grp_pullback_pr1 _ _ $o (grp_iso_inverse p.1) $o ab_biprod_inr)).
+  1,2: exact _. (* Why doesn't Coq find Group's [Is01Cat] instance? *)
+  nrapply (istruncmap_compose _ (grp_iso_inverse p.1 o ab_biprod_inr)).
+  all : rapply istruncmap_mapinO_tr.
+Defined.
+
+Definition abses_pullback_inclusion_transpose_endpoint' `{Univalence} {A B E : AbGroup}
+           (i : B $-> E) `{IsEmbedding i}
+           (F : AbSES E A) (p : abses_pullback0 i F $== point _)
+  : AbGroup := QuotientAbGroup F (abses_pullback_inclusion_transpose_subgroup i F p).
+
+(** By [abses_from_inclusion] we get a short exact sequence [B -> F -> F/B] associated to the subgroup and quotient just above. *)
+
+Lemma abses_pullback_inclusion_transpose_beta `{Univalence} {A B E : AbGroup}
+      (i : B $-> E) `{IsEmbedding i}
+      (F : AbSES E A) (p : abses_pullback0 i F $== point _)
+  : projection F $o (grp_pullback_pr1 (projection F) _ $o p^$.1 $o ab_biprod_inr) == i.
+Proof.
+  rapply (conn_map_elim _ (ab_biprod_pr2 (A:=A))).
+  intro ab.
+  refine (pullback_commsq _ _ _ @ ap i _).
+  exact (snd p^$.2 _)^.
+Defined.
+
+(** Short exact sequences in the fiber of [inclusion E] descend along [projection E]. *)
+Definition abses_pullback_trivial_preimage `{Univalence} {A B C : AbGroup} (E : AbSES C B)
+           (F : AbSES (middle E) A) (p : abses_pullback0 (inclusion E) F $== point _)
+  : AbSES C A.
+Proof.
+  snrapply Build_AbSES.
+  - exact (abses_pullback_inclusion_transpose_endpoint' (inclusion E) F p).
+  - exact (grp_quotient_map $o inclusion F).
+  - snrapply grp_quotient_rec.
+    + exact (projection E $o projection F).
+    + intros f [b q].
+      rewrite <- q.
+      refine (ap (projection E) (abses_pullback_inclusion_transpose_beta (inclusion E) F p b) @ _).
+      apply iscomplex_abses.
+  - apply isembedding_grouphomomorphism.
+    intros a q0.
+    (* Since [inclusion F a] is killed by [grp_quotient_map], its in the image of [B]. *)
+    assert (in_coset :  in_cosetL (abses_pullback_inclusion_transpose_subgroup (inclusion E) F p)
+                           (inclusion F a) mon_unit). (** todo: consider not using inclusion here, but grp_pullback_pr1 *)
+    1:{ rapply related_quotient_paths.
+        exact q0. }
+    (* Cleaning up the context facilitates later steps. *)
+    destruct in_coset as [b q1]; rewrite grp_unit_r in q1.
+    (* Since both [inclusion F] and [B -> F] factor through the mono [ab_biprod A B -> F], we can lift [q1] to [ab_biprod A B]. *)
+    assert (q2 : ab_biprod_inr  b = ab_biprod_inl (-a)).
+    1: { apply (isinj_embedding (grp_pullback_pr1 _ _ $o p^$.1)).
+         - nrapply (istruncmap_compose (-1) p^$.1 (grp_pullback_pr1 (projection F) (inclusion E))).
+           all: rapply istruncmap_mapinO_tr.
+         - nrefine (q1 @ _); symmetry.
+           refine (ap (grp_pullback_pr1 _ _) (fst p^$.2 (-a)) @ _).
+           exact (grp_homo_inv _ _). }
+    (* Using [q2], we conclude. *)
+    pose proof (q3 := ap (-) (fst ((equiv_path_prod _ _)^-1 q2))); cbn in q3.
+    exact ((negate_involutive _)^ @ q3^ @ negate_mon_unit).
+  - rapply (cancelR_conn_map (Tr (-1)) grp_quotient_map).
+    rapply conn_map_homotopic.
+    reflexivity.
+  - srapply Build_IsExact.
+    + srapply Build_pHomotopy.
+      * intro a; simpl.
+        refine (ap (projection E) _ @ _).
+        1: apply iscomplex_abses.
+        apply grp_homo_unit.
+      * apply path_ishprop.
+    + intros [y q].
+      rapply contr_inhabited_hprop.
+      (* We choose a preimage by [grp_quotient_map]. *)
+      assert (f : merely (hfiber grp_quotient_map y)).
+      1: apply center, issurj_class_of. (* todo: clean up *)
+      strip_truncations; destruct f as [f q0].
+      (* Since [projection F f] is in the kernel of [projection E], we find a preimage in [B]. *)
+      assert (b : merely (hfiber (inclusion E) (projection F f))).
+      1: { rapply isexact_preimage.
+           exact (ap _ q0 @ q). }
+      strip_truncations; destruct b as [b q1].
+      (* The difference [f - b] in [F] is in the kernel of [projection F], hence lies in [A]. *)
+      assert (a : merely (hfiber (inclusion F)
+                                 (sg_op f (-(grp_pullback_pr1 _ _ (p^$.1 (ab_biprod_inr b))))))).
+      1: { rapply isexact_preimage.
+           refine (grp_homo_op _ _ _ @ _).
+           refine (ap (fun x => _ + x) (grp_homo_inv _ _) @ _).
+           refine (ap (fun x => _ - x) (abses_pullback_inclusion_transpose_beta (inclusion E) F p b @ q1) @ _).
+           apply right_inverse. }
+      strip_truncations; destruct a as [a q2].
+      (* It remains to show that [a] is the desired preimage. *)
+      refine (tr (a; _)).
+      apply path_sigma_hprop.
+      refine (ap grp_quotient_map q2 @ _ @ q0).
+      refine (grp_homo_op _ _ _ @ _).
+      apply grp_moveR_Mg.
+      refine (_ @ (left_inverse _)^).
+      apply qglue.
+      exists b.
+      refine (_ @ (grp_unit_r _)^).
+      exact (negate_involutive _)^.
+Defined.
+
+(** That [abses_pullback_trivial_preimage E F p] pulls back to [F] is immediate [abses_component1_trivial_pullback] and the following map: *)
+
+Definition abses_pullback_inclusion0_map' `{Univalence} {A B C : AbGroup} (E : AbSES C B)
+           (F : AbSES (middle E) A) (p : abses_pullback0 (inclusion E) F $== point _)
+  : AbSESMorphism F (abses_pullback_trivial_preimage E F p).
+Proof.
+  srapply Build_AbSESMorphism.
+  - exact grp_homo_id.
+  - exact grp_quotient_map.
+  - exact (projection E).
+  - reflexivity.
+  - reflexivity.
+Defined.
+
+(** Of course, we need not only a preimage of [F] but a preimage of [(F,p)] along [cxfib]. We now define and prove this in terms of path data. *)
+
+(** The analog of [cxfib] induced by pullback in terms of path data. *)
+Definition cxfib' `{Funext} {A B C : AbGroup} (E : AbSES C B)
+  : AbSES C A -> hfiber_abses (A:=A) (abses_pullback0 (inclusion E)) (point _).
+Proof.
+  intro Y.
+  exists (abses_pullback0 (projection E) Y).
+  refine (abses_pullback_compose' _ _ Y $@ _).
+  refine (abses_pullback_homotopic' _ grp_homo_const _ Y $@ _).
+  1: rapply iscomplex_abses.
+  symmetry; apply abses_pullback_const'.
+Defined.
+
+Definition hfiber_cxfib' `{Funext} {A B C : AbGroup} (E : AbSES C B)
+           (F : AbSES (middle E) A) (p : abses_pullback0 (inclusion E) F $== point _)
+  := {Y : AbSES C A & hfiber_abses_path (cxfib' E Y) (F; p)}.
+
+Definition equiv_hfiber_cxfib' `{Univalence} {A B C : AbGroup} {E : AbSES C B}
+           (F : AbSES (middle E) A) (p : abses_pullback0 (inclusion E) F $== point _)
+  : hfiber_cxfib' E F p <~> hfiber (cxfib (iscomplex_pullback_abses E))
+                  (equiv_hfiber_abses _ (point _) (F;p)).
+Proof.
+  srapply equiv_functor_sigma_id; intro U; lazy beta.
+  refine (_ oE equiv_hfiber_abses_pullback _ _ _).
+  refine (_ oE equiv_ap' (equiv_hfiber_abses _ (point _)) _ _).
+  apply equiv_concat_l.
+  srapply path_sigma.
+  1: reflexivity.
+  nrefine (transport_1 _ _ @ _).
+  unfold cxfib, Build_pMap, pointed_fun, pr2,
+    iscomplex_pullback_abses, phomotopy_transitive,
+    Build_pHomotopy, pointed_fun.
+  nrefine (concat_p1 _ @ _).
+  nrefine (concat_1p _ @ _).
+  (* [reflexivity.] works here, but is too slow. *)
+  nrapply (ap equiv_path_abses_iso).
+  rapply path_hom.
+  snrapply (fmap (cat_comp ((abses_pullback_pconst'.1 U)^$ $o (abses_pullback_homotopic' _ _ _) U))).
+  3: apply Id.
+  rapply is0functor_postcomp.
+Defined.
+
+(** The type of paths in [hfiber_cxfib'] in terms of path data. *)
+Definition path_hfiber_cxfib' `{Funext} {A B C : AbGroup} {E : AbSES C B}
+           {F : AbSES (middle E) A} {p : abses_pullback0 (inclusion E) F $== point _}
+           (X Y : hfiber_cxfib' (B:=B) E F p)
+  : Type.
+Proof.
+  refine (sig (fun q0 : X.1 $== Y.1 => _)).
+  exact ((fmap (abses_pullback0 (projection E)) q0)^$ $@ X.2.1 $== Y.2.1).
+Defined.
+
+Definition transport_hfiber_abses_path_cxfib'_l `{Univalence} {A B C : AbGroup} {E : AbSES C B}
+           (F : AbSES (middle E) A) (p : abses_pullback0 (inclusion E) F $== point _)
+           (U V : hfiber_cxfib' E F p) (q : U.1 = V.1)
+  : (transport (fun Y : AbSES C A => hfiber_abses_path (cxfib' E Y) (F; p)) q U.2).1
+    = fmap (abses_pullback0 (projection E)) (equiv_path_abses_iso^-1 q^) $@ U.2.1.
+Proof.
+  induction q.
+  refine (ap pr1 (transport_1 _ _) @ _).
+  refine (_ @ ap (fun x => fmap (abses_pullback0 (projection E)) x $@ _) equiv_path_absesV_1^).
+  refine (_ @ ap (fun x => x $@ _) (fmap_id_strong _ _)^).
+  exact (cat_idr_strong _)^.
+Defined.
+
+Definition equiv_path_hfiber_cxfib' `{Univalence} {A B C : AbGroup} {E : AbSES C B}
+           (F : AbSES (middle E) A) (p : abses_pullback0 (inclusion E) F $== point _)
+           (U V : hfiber_cxfib' E F p)
+  : path_hfiber_cxfib' U V <~> U = V.
+Proof.
+  refine (equiv_path_sigma _ _ _ oE _).
+  srapply (equiv_functor_sigma' equiv_path_abses_iso);
+    intro q; lazy beta.
+  refine (equiv_path_sigma_hprop _ _ oE _).
+  refine (equiv_concat_l _ _ oE _).
+  1: apply transport_hfiber_abses_path_cxfib'_l.
+  refine (equiv_path_sigma_hprop _ _ oE equiv_concat_l _ _ oE _).
+  1: { refine (ap (fun x => (fmap (abses_pullback0 _) x $@ _).1) _).
+       nrefine (ap _ (abses_path_data_V q) @ _).
+       apply eissect. }
+  refine (equiv_concat_l _ _ oE _).
+  1: { refine (ap (fun x => (x $@ _).1) _).
+       rapply gpd_strong_1functor_V. }
+  apply equiv_path_groupisomorphism.
+Defined.
+
+(** The fibre of [cxfib'] over [(F;p)] is inhabited. *)
+Definition hfiber_cxfib'_inhabited `{Univalence} {A B C : AbGroup} (E : AbSES C B)
+      (F : AbSES (middle E) A) (p : abses_pullback (inclusion E) F $== point _)
+  : hfiber_cxfib' E F p.
+Proof.
+  exists (abses_pullback_trivial_preimage E F p).
+  srefine (_; _).
+  1: symmetry; by nrapply (abses_component1_trivial_pullback' (abses_pullback_inclusion0_map' E F p)).
+  lazy beta; unfold pr2.
+  refine (cat_assoc _ _ _ $@ _).
+  refine (cat_assoc _ _ _ $@ _).
+  apply gpd_moveR_Vh.
+  apply gpd_moveL_hM.
+  apply equiv_path_biprod_corec.
+  split; apply equiv_path_pullback_rec_hset; split; cbn.
+  - intro a.
+    refine (ap (class_of _) _).
+    exact (ap pullback_pr1 (fst p^$.2 a)).
+  - intro a.
+    exact ((snd p^$.2 _)^).
+  - intro b; apply qglue.
+    exists (-b).
+    apply grp_moveL_Vg.
+    refine ((grp_homo_op (grp_pullback_pr1 _ _ $o p^$.1 $o ab_biprod_inr) _ _)^ @ _).
+    exact (ap _ (right_inverse _) @ grp_homo_unit _ @ (grp_homo_unit _)^).
+  - intro b. cbn.
+    exact ((snd p^$.2 _)^).
+Defined.
+
+(** To conclude exactness in terms of path data, we show that the fibre is a proposition, hence contractible. *)
+
+(** Given a point [(Y;Q)] in the fiber of [cxfib'] over [(F;p)] there is an induced map as follows. *)
+Local Definition hfiber_cxfib'_induced_map `{Funext} {A B C : AbGroup} (E : AbSES C B)
+      (F : AbSES (middle E) A) (p : abses_pullback0 (inclusion E) F $== point _)
+      (Y : hfiber_cxfib' E F p)
+  : ab_biprod A B $-> abses_pullback0 (projection E) Y.1.
+Proof.
+  destruct Y as [Y q].
+  refine (grp_homo_compose _ (grp_iso_inverse p.1)).
+  refine (_ $o grp_pullback_pr1 _ _).
+  exact (q.1^$.1).
+Defined.
+
+(** There is "another" obvious induced map. *)
+Definition abses_pullback_splits_induced_map' {A B C : AbGroup}
+           (E : AbSES C B) (Y : AbSES C A)
+  : ab_biprod A B $-> abses_pullback0 (projection E) Y.
+Proof.
+  srapply (ab_biprod_rec (inclusion _)).
+  srapply grp_pullback_corec.
+  - exact grp_homo_const.
+  - exact (inclusion E).
+  - intro x.
+    refine (grp_homo_unit _ @ _).
+    symmetry; apply iscomplex_abses.
+Defined.
+
+Lemma fmap_hfiber_abses_lemma `{Univalence} {A B B' : AbGroup} (f : B' $-> B)
+           (X Y : hfiber_abses (abses_pullback0 (A:=A) f) (point _)) (Q : hfiber_abses_path X Y)
+  : fmap (abses_pullback0 f) Q.1^$ $o Y.2^$ $== X.2^$.
+Proof.
+  generalize Q.
+  equiv_intro (equiv_hfiber_abses_pullback _ X Y)^-1%equiv p;
+    induction p.
+  refine ((_ $@R _) $@ _).
+  { Unshelve.
+    2: exact (Id _).
+    refine (fmap2 _ _ $@ fmap_id _ _).
+    intro x; reflexivity. }
+  exact (cat_idl _).
+Defined.
+
+Lemma induced_map_eq `{Univalence} {A B C : AbGroup} (E : AbSES C B)
+      (F : AbSES (middle E) A) (p : abses_pullback0 (inclusion E) F $== point _)
+      (Y : hfiber_cxfib' E F p)
+  : hfiber_cxfib'_induced_map E F p Y == abses_pullback_splits_induced_map' E Y.1.
+Proof.
+  intros [a b]; cbn.
+  refine (ap pullback_pr1 (fmap_hfiber_abses_lemma _ _ (F;p) Y.2 _) @ _).
+  srapply equiv_path_pullback_hset; split; cbn.
+  - exact (grp_unit_r _)^.
+  - exact (grp_unit_l _)^.
+Defined.
+
+(** Given another point [(Y,Q)] in the fibre of [cxfib'] over [(F;p)], we get path data in [AbSES C A]. *)
+Lemma hfiber_cxfib'_induced_path'0 `{Univalence} {A B C : AbGroup} (E : AbSES C B)
+      (F : AbSES (middle E) A) (p : abses_pullback0 (inclusion E) F $== point _)
+      (Y : hfiber_cxfib' E F p)
+  : abses_pullback_trivial_preimage E F p $== Y.1.
+Proof.
+  destruct Y as [Y Q].
+  apply equiv_path_abses_data;
+    srefine (_; (_,_)).
+  - srapply grp_quotient_rec.
+    1: exact (grp_pullback_pr1 _ _$o (Q.1^$).1).
+    intros f [b q0].
+    refine (ap _ q0^ @ _).
+    nrefine (ap _ (induced_map_eq E F p (Y;Q) _) @ _); cbn.
+    exact (grp_unit_r _ @ grp_homo_unit _).
+  - intro a.
+    refine (_ @ ap (grp_pullback_pr1 _ _) (fst (Q.1^$).2 a)).
+    exact (grp_quotient_rec_beta' _ F _ _ (inclusion F a)).
+  - rapply (conn_map_elim _ grp_quotient_map); intro f.
+    refine (ap (projection E) (snd (Q.1^$).2 f) @ _); unfold pr1.
+    exact (pullback_commsq _ _ ((Q.1^$).1 f))^.
+Defined.
+
+Lemma hfiber_cxfib'_induced_path' `{Univalence} {A B C : AbGroup} (E : AbSES C B)
+      (F : AbSES (middle E) A) (p : abses_pullback0 (inclusion E) F $== point _)
+      (Y : hfiber_cxfib' E F p)
+  : path_hfiber_cxfib' (hfiber_cxfib'_inhabited E F p) Y.
+Proof.
+  exists (hfiber_cxfib'_induced_path'0 E F p Y).
+  rapply gpd_moveR_Vh.
+  rapply gpd_moveL_hM.
+  rapply gpd_moveR_Vh.
+  intro x.
+  srapply equiv_path_pullback_hset; split.
+  2: exact (snd Y.2.1^$.2 x)^.
+  reflexivity.
+Defined.
+
+(** It follows that [hfiber_cxfib'] is contractible. *)
+Lemma contr_hfiber_cxfib' `{Univalence} {A B C : AbGroup} (E : AbSES C B)
+      (F : AbSES (middle E) A) (p : abses_pullback0 (inclusion E) F $== point _)
+  : Contr (hfiber_cxfib' E F p).
+Proof.
+  srapply Build_Contr.
+  1: apply hfiber_cxfib'_inhabited.
+  intros [Y q].
+  apply equiv_path_hfiber_cxfib'.
+  apply hfiber_cxfib'_induced_path'.
+Defined.
+
+(** From this we deduce exactness. *)
+Global Instance isexact_abses_pullback `{Univalence} {A B C : AbGroup} {E : AbSES C B}
+  : IsExact purely (abses_pullback (A:=A) (projection E)) (abses_pullback (inclusion E)).
+Proof.
+  srapply Build_IsExact.
+  1: apply iscomplex_pullback_abses.
+  srapply (equiv_ind (equiv_hfiber_abses (abses_pullback0 (inclusion E)) (point (AbSES B A)))).
+  intros [F p].
+  rapply contr_equiv'.
+  1: apply equiv_hfiber_cxfib'.
+  apply contr_hfiber_cxfib'.
+Defined.
